\documentclass[12pt]{article}
\usepackage{amssymb}
\usepackage{amsmath}
\usepackage[margin=1.2in]{geometry}
\usepackage[most]{tcolorbox}
\usepackage{footnotebackref}
\usepackage{tikz}
\newcommand{\thm}[3]{\begin{tcolorbox}[title=\textbf{Theorem #1: #2},
coltitle=black,colback=blue!20, colframe=blue!50]#3\end{tcolorbox}}
\newcommand{\df}[3]{\begin{tcolorbox}[title=\textbf{Definition #1: #2},
coltitle=black,colback=red!20, colframe=red!40]#3\end{tcolorbox}}
\newcommand{\ex}[2]{\begin{tcolorbox}[title=\textbf{Example #1},
coltitle=black,colback=green!20, colframe=green!50]#2\end{tcolorbox}}
\newcommand{\N}{\mathbb{N}}
\newcommand{\Z}{\mathbb{Z}}
\newcommand{\Q}{\mathbb{Q}}
\newcommand{\R}{\mathbb{R}}
\newcommand{\C}{\mathbb{C}}
\newcommand{\T}{\mathcal{T}}
\newcommand{\pf}{\textit{Proof. }}
\newcommand{\lm}{\textit{Lemma. }}
\newcommand{\nn}{\\[0.5em]}
\newcommand{\nl}{\\[1.0em]}
\newcommand{\ep}{\hfill $\blacksquare$\nl}
\newcommand{\ec}{\hfill $\square$\nn}
\newcommand{\quot}[2]{\textit{``#1"} $\sim$ \textbf{#2}\nl}
\newcommand{\start}[1]{
\LARGE \centering #1 \nl
\normalsize \raggedright
}
\begin{document}
\setlength\parskip{0.5em minus 0.2em}
\[z = wx + b\]
\[y = \dfrac{1}{1 + e^{-z}}\]
\[\mathcal{L}(y,t) = -t\log(y) + (t-1)\log(1-y)\]
\[\dfrac{\partial \mathcal{L}}{\partial y}
= \dfrac{-t}{y} + \dfrac{t-1}{1-y}\]
\[\dfrac{dy}{dz} = \dfrac{e^{-z}}{(1 + e^{-z})^2}\]
\[\dfrac{\partial z}{\partial w}
= x\]
\[\Rightarrow 
\dfrac{\partial \mathcal{L}}{\partial w}
= \left(\dfrac{-t}{y}
+ \dfrac{t-1}{1-y}\right)
\left(\dfrac{e^{-z}}{(1+e^{-z})^2}\right)x\]
\[\Rightarrow 
\dfrac{\partial \mathcal{L}}{\partial b}
= \left(\dfrac{-t}{y}
+ \dfrac{t-1}{1-y}\right)
\left(\dfrac{e^{-z}}{(1+e^{-z})^2}\right)
\]

\end{document}
